Finished first pset.

pset01_ProgramAnalysis/Pset1.v
@@ -1,6 +1,7 @@
 (** * 6.822 Formal Reasoning About Programs, Spring 2020 - Pset 1 *)
 
 Require Import Frap Pset1Sig.
+Require Import Nat.
 
 (* The first part of this assignment involves the [bool] datatype,
  * which has the following definition.
@@ -16,8 +17,11 @@ Require Import Frap Pset1Sig.
 (* Define [Neg] so that it implements Boolean negation, which flips
  * the truth value of a Boolean value.
  *)
-Definition Neg (b : bool) : bool.
-Admitted.
+Definition Neg (b : bool) : bool :=
+  match b with
+  | true => false
+  | false => true
+  end.
 
 (* For instance, the negation of [true] should be [false].
  * This proof should follow from reducing both sides of the equation
@@ -25,7 +29,9 @@ Admitted.
  *)
 Theorem Neg_true : Neg true = false.
 Proof.
-Admitted.
+  simplify.
+  equality.
+Qed.
 
 (* Negation should be involutive, meaning that if we negate
  * any Boolean value twice, we should get the original value back.
@@ -36,39 +42,69 @@ Admitted.
  *)
 Theorem Neg_involutive : forall b : bool, Neg (Neg b) = b.
 Proof.
-Admitted.
+  simplify.
+  cases b.
+  equality.
+  equality.
+Qed.
 
 (* Define [And] so that it implements Boolean conjunction. That is,
  * the result value should be [true] exactly when both inputs
  * are [true].
  *)
-Definition And (x y : bool) : bool.
-Admitted.
+Definition And (x y : bool) : bool :=
+  match x with
+  | true
+    => match y with
+    | true => true
+    | false => false
+    end
+  | false =>  false
+  end.
 
 (* Here are a couple of examples of how [And] should act on
  * concrete inputs.
  *)
 Theorem And_true_true : And true true = true.
 Proof.
-Admitted.
+  equality.
+Qed.
 
 Theorem And_false_true : And false true = false.
 Proof.
-Admitted.
+  equality.
+Qed.
 
 (* Prove that [And] is commutative, meaning that switching the order
  * of its arguments doesn't affect the result.
  *)
 Theorem And_comm : forall x y : bool, And x y = And y x.
 Proof.
-Admitted.
+  simplify.
+
+  cases x.
+
+  cases y.
+
+  equality.
+  equality.
+
+  cases y.
+
+  equality.
+  equality.
+Qed.
 
 (* Prove that the conjunction of a Boolean value with [true]
  * doesn't change that value.
  *)
 Theorem And_true_r : forall x : bool, And x true = x.
 Proof.
-Admitted.
+  simplify.
+  cases x.
+  equality.
+  equality.
+Qed.
 
 (* In the second part of this assignment, we will work with a simple language
  * of imperative arithmetic programs that sequentially apply operations
@@ -83,43 +119,69 @@ Print Prog.
  * that running the program [p] should result in, when the
  * initial state is [n].
  *)
-Fixpoint run (p : Prog) (initState : nat) : nat.
-Admitted.
+Fixpoint run (p : Prog) (initState : nat) : nat :=
+  match p with
+  | Done => initState
+  | AddThen val p_remaining => run p_remaining (val + initState)
+  | MulThen val p_remaining => run p_remaining (val * initState)
+  | DivThen val p_remaining => run p_remaining (initState / val)
+  | VidThen val p_remaining => run p_remaining (val / initState)
+  | SetToThen val p_remaining => run p_remaining val
+  end.
 
 Theorem run_Example1 : run Done 0 = 0.
 Proof.
-Admitted.
+  equality.
+Qed.
 
 Theorem run_Example2 : run (MulThen 5 (AddThen 2 Done)) 1 = 7.
 Proof.
-Admitted.
+  equality.
+Qed.
 
 Theorem run_Example3 : run (SetToThen 3 (MulThen 2 Done)) 10 = 6.
 Proof.
-Admitted.
+  equality.
+Qed.
 
 (* Define [numInstructions] to compute the number of instructions
  * in a program, not counting [Done] as an instruction.
  *)
-Fixpoint numInstructions (p : Prog) : nat.
-Admitted.
+Fixpoint numInstructions (p : Prog) : nat :=
+  match p with
+  | Done => 0
+  | AddThen _ p_remaining => 1 + (numInstructions p_remaining)
+  | MulThen _ p_remaining => 1 + (numInstructions p_remaining)
+  | DivThen _ p_remaining => 1 + (numInstructions p_remaining)
+  | VidThen _ p_remaining => 1 + (numInstructions p_remaining)
+  | SetToThen _ p_remaining => 1 + (numInstructions p_remaining)
+  end.
 
 Theorem numInstructions_Example :
   numInstructions (MulThen 5 (AddThen 2 Done)) = 2.
 Proof.
-Admitted.
+  equality.
+Qed.
 
 (* Define [concatProg] such that [concatProg p1 p2] is the program
  * that first runs [p1] and then runs [p2].
  *)
-Fixpoint concatProg (p1 p2 : Prog) : Prog.
-Admitted.
+Fixpoint concatProg (p1 p2 : Prog) : Prog :=
+  match p1 with
+  | Done => p2
+  | AddThen   val p1_rem => AddThen val (concatProg p1_rem p2)
+  | MulThen   val p1_rem => MulThen val (concatProg p1_rem p2)
+  | DivThen   val p1_rem => DivThen val (concatProg p1_rem p2)
+  | VidThen   val p1_rem => VidThen val (concatProg p1_rem p2)
+  | SetToThen val p1_rem => SetToThen val (concatProg p1_rem p2)
+  end.
 
 Theorem concatProg_Example :
      concatProg (AddThen 1 Done) (MulThen 2 Done)
      = AddThen 1 (MulThen 2 Done).
 Proof.
-Admitted.
+  equality.
+Qed.
 
 (* Prove that the number of instructions in the concatenation of
  * two programs is the sum of the number of instructions in each
@@ -129,7 +191,16 @@ Theorem concatProg_numInstructions
   : forall (p1 p2 : Prog), numInstructions (concatProg p1 p2)
                       = numInstructions p1 + numInstructions p2.
 Proof.
-Admitted.
+  simplify.
+  induct p1.
+
+  simplify; equality.
+  simplify; equality.
+  simplify; equality.
+  simplify; equality.
+  simplify; equality.
+  simplify; equality.
+Qed.
 
 (* Prove that running the concatenation of [p1] with [p2] is
    equivalent to running [p1] and then running [p2] on the
@@ -139,7 +210,16 @@ Theorem concatProg_run
     run (concatProg p1 p2) initState =
     run p2 (run p1 initState).
 Proof.
-Admitted.
+  simplify.
+  induct p1.
+  simplify; equality.
+
+  apply IHp1.
+  apply IHp1.
+  apply IHp1.
+  apply IHp1.
+  apply IHp1.
+Qed.
 
 (* Read this definition and understand how division by zero is handled. *)
 Fixpoint runPortable (p : Prog) (state : nat) : bool * nat :=
@@ -164,7 +244,31 @@ Arguments Nat.div : simpl never. (* you don't need to understand this line *)
 Lemma runPortable_run : forall p s0 s1,
   runPortable p s0 = (true, s1) -> run p s0 = s1.
 Proof.
-Admitted.
+  simplify.
+  induct p.
+
+  simplify; equality.
+  apply IHp; equality.
+  apply IHp; equality.
+
+  cases  n.
+  simplify;  equality.
+  apply IHp.
+  simplify; equality.
+
+  cases  n.
+  apply IHp.
+  simplify.
+  cases s0.
+  simplify; equality.
+  simplify; equality.
+  simplify.
+  cases s0.
+  simplify; equality.
+  simplify; apply IHp; equality.
+
+  simplify; apply IHp; equality.
+Qed.
 
 
 (* The final goal of this pset is to implement [validate : Prog -> bool]
@@ -203,16 +307,37 @@ Definition goodProgram7 := AddThen 1 (DivThen 1 (DivThen 1 (VidThen 1 Done))).
  * and one intermediate lemma in the soundness proof -- both of which are more
  * sophisticated than the top-level versions given here. *)
 
-Definition validate (p : Prog) : bool.
-Admitted.
+Fixpoint validate_helper (p : Prog) (possible_zero : bool) : bool :=
+  match p with
+  | Done => true
+  | AddThen n p' => validate_helper p' (if possible_zero then (if n ==n 0 then true else false) else false)
+  | MulThen n p' => validate_helper p' (if n ==n 0 then true else possible_zero)
+  | DivThen n p' => if n ==n 0 then false else validate_helper p' (if n ==n 1 then possible_zero else true)
+  | VidThen n p' => if possible_zero then false else validate_helper p' true
+  | SetToThen n p' => validate_helper p' (if n ==n 0 then true else false)
+  end.
 
-Example validate1 : validate goodProgram1 = true. Admitted.
-Example validate2 : validate goodProgram2 = true. Admitted.
-Example validate3 : validate goodProgram3 = true. Admitted.
-Example validate4 : validate goodProgram4 = true. Admitted.
-Example validate5 : validate goodProgram5 = true. Admitted.
-Example validate6 : validate goodProgram6 = true. Admitted.
-Example validate7 : validate goodProgram7 = true. Admitted.
+Definition validate (p : Prog) : bool := validate_helper p true.
+
+Example validate1 : validate goodProgram1 = true.
+Proof.  simplify.  equality.  Qed.
+Example validate2 : validate goodProgram2 = true.
+Proof.  simplify.  equality.  Qed.
+Example validate3 : validate goodProgram3 = true.
+Proof.  simplify.  equality.  Qed.
+Example validate4 : validate goodProgram4 = true.
+Proof.  simplify.  equality.  Qed.
+Example validate5 : validate goodProgram5 = true.
+Proof.  simplify.  equality.  Qed.
+Example validate6 : validate goodProgram6 = true.
+Proof.  simplify.  equality.  Qed.
+Example validate7 : validate goodProgram7 = true.
+Proof.  simplify.  equality.  Qed.
+
+Example validateBad1 : validate badProgram1 = false.
+Proof.  simplify. equality. Qed.
+Example validateBad2 : validate badProgram2 = false.
+Proof.  simplify. equality. Qed.
 
 (* If a clear plan hasn't emerged in 10 minutes (or if you get stuck later),
  * take a look at the hints for this pset on the course web site.
@@ -225,9 +350,146 @@ Example validate7 : validate goodProgram7 = true. Admitted.
  * necessary, and only jump into coding when you have some idea why it should
  * succeed. Some may call Coq a video game, but it is not a grinding contest. *)
 
+Lemma temp : forall (s : nat), s <> 0 -> forall n, s + n * s <> 0.
+Proof.
+  simplify.
+  apply Nat.neq_0_lt_0 in H.
+  apply Nat.neq_0_lt_0.
+  Search(0 < _ -> 0 < _ + _).
+  apply Nat.add_pos_l with (n := s).
+  equality.
+Qed.
+
+
+Lemma validate_helper_sound : forall p possible_zero, validate_helper p possible_zero = true ->
+  forall s, ((possible_zero = false -> (s <> 0)))
+  -> runPortable p s = (true, run p s).
+Proof.
+  simplify.
+  induct p.
+  induct s.
+
+  simplify; equality.
+  simplify; equality.
+
+  simplify.
+  cases possible_zero.
+    cases n.
+      simplify.
+      apply IHp with (possible_zero := true).
+      equality.
+      equality.
+      simplify.
+      apply IHp with (possible_zero := false).
+      equality.
+      equality.
+    cases n.
+      simplify.
+      apply IHp with (possible_zero := false).
+      equality.
+      equality.
+      simplify.
+      apply IHp with (possible_zero := false).
+      equality.
+      equality.
+
+  simplify.
+  cases possible_zero.
+    cases n.
+      simplify.
+      apply IHp with (possible_zero := true).
+      equality.
+      equality.
+      simplify.
+      apply IHp with (possible_zero := true).
+      equality.
+      propositional.
+      equality.
+    cases n.
+      simplify.
+      apply IHp with (possible_zero := true).
+      equality.
+      equality.
+      propositional.
+      simplify.
+      apply IHp with (possible_zero := false).
+      equality.
+      propositional.
+      apply temp with (n:= n) in H1.
+      equality.
+
+  simplify.
+    cases possible_zero.
+      cases n.
+        simplify.
+        equality.
+        simplify.
+      cases n.
+        simplify.
+        rewrite Nat.div_1_r with (a := s).
+        apply IHp with (possible_zero := true).
+        equality.
+        equality.
+        simplify.
+        apply IHp with (possible_zero := true).
+        equality.
+        equality.
+        propositional.
+      cases n.
+        simplify.
+        equality.
+        simplify.
+        cases n.
+          simplify.
+          apply IHp with (possible_zero := false).
+          equality.
+          rewrite Nat.div_1_r with (a := s).
+          equality.
+          simplify.
+          propositional.
+          apply IHp with (possible_zero := true).
+          equality.
+          equality.
+
+  simplify.
+  cases possible_zero.
+    cases s.
+      equality.
+      equality.
+    propositional.
+    cases (n / s).
+      cases s.
+        equality.
+        simplify.
+        apply IHp with (possible_zero := true).
+        equality.
+        equality.
+      cases s.
+        equality.
+        simplify.
+        apply IHp with (possible_zero := true).
+        equality.
+        equality.
+
+  cases n.
+    simplify.
+    apply IHp with (possible_zero := true).
+    equality.
+    equality.
+    simplify.
+    apply IHp with (possible_zero := false).
+    equality.
+    equality.
+Qed.
+
 Lemma validate_sound : forall p, validate p = true ->
   forall s, runPortable p s = (true, run p s).
-Admitted.
+Proof.
+  simplify.
+  apply validate_helper_sound with (possible_zero := true).
+  equality.
+  equality.
+Qed.
 
 (* Here is the complete list of commands used in one possible solution:
   - Search, for example Search (_ + 0).
